check

coq/two/LambdaTwo.v
@@ -1,51 +1,97 @@
+Require Import Omega.
+Require Import Recdef.
 Require Export LambdaTwoSyntax.
 Require Export IndistinguishabilityTwo.
 
-Fixpoint eval_k (k : nat) (L : two) (P : value -> value -> Prop)
-         (pc : two) (e : env) (t : term) (a : atom)
-         {struct k} : Prop :=
-  match t with
-    | TBool b =>
-      a = Atom (VBool b) pc
-    | TNat n =>
-      a = Atom (VNat n) pc
-    | TVar n =>
-      exists v l,
-        atIndex e n = Some (Atom v l) /\
-        a = Atom v (l ⊔ pc)
-    | TAbs t' =>
-      a = Atom (VClos e t') pc
-    | TApp t1 t2 =>
-      match k with
-        | S k' =>
-          exists e1' t1' l1 a2 a3,
-            eval_k k' L P pc e t1 (Atom (VClos e1' t1') l1) /\
-            eval_k k' L P pc e t2 a2 /\
-            eval_k k' L P l1 (a2 :: e1') t1' a3 /\
-            a = a3
-        | 0 => False
-      end
-    | TDecl t1 t2 =>
-      match k with
-        | S k' =>
+Definition pair_add (a : nat * nat) : nat :=
+  match a with
+    | (a1, a2) => a1 + a2
+  end.
+
+Definition pair_lt (a b : nat * nat) : Prop :=
+  pair_add a < pair_add b.
+
+Lemma pair_lt_wf' :
+  forall s a, pair_add a <= s -> Acc pair_lt a.
+Proof.
+  induction s; intros a H1.
+  - destruct a as [a1 a2]; destruct a1; destruct a2; auto.
+    apply Acc_intro. intros y H2. inversion H2.
+  - inversion H1 as [H2 | n H2 Heq]; auto.
+    apply Acc_intro. intros y H3. inversion H3; auto.
+Defined.
+
+Theorem pair_lt_wf : well_founded pair_lt.
+Proof.
+  unfold well_founded; intro; eapply pair_lt_wf'; eauto.
+Defined.
+
+Definition eval_kl : nat * nat -> two -> (value -> value -> Prop) ->
+                     two -> env -> term -> atom -> Prop.
+  refine
+    (Fix pair_lt_wf (fun _ => two -> (value -> value -> Prop) ->
+                              two -> env -> term -> atom -> Prop)
+         (fun (kl : nat * nat)
+              (eval_kl : forall kl' : nat * nat,
+                           pair_lt kl' kl ->
+                           two -> (value -> value -> Prop) ->
+                           two -> env -> term -> atom -> Prop) =>
+            fun (L : two) (P : value -> value -> Prop)
+                (pc : two) (e : env) (t : term) (a : atom) =>
+              match t with
+                | TBool b =>
+                  a = Atom (VBool b) pc
+                | TNat n =>
+                  a = Atom (VNat n) pc
+                | TVar n =>
+                  exists v l,
+                    atIndex e n = Some (Atom v l) /\
+                    a = Atom v (l ⊔ pc)
+                | TAbs t' =>
+                  a = Atom (VClos e t') pc
+                | TApp t1 t2 =>
+                  if Compare_dec.zerop (fst kl) then False
+                  else exists e1' t1' l1 a2 a3,
+                         eval_kl (fst kl - 1, snd kl) _
+                                 L P pc e t1 (Atom (VClos e1' t1') l1) /\
+                         eval_kl (fst kl - 1, snd kl) _
+                                 L P pc e t2 a2 /\
+                         eval_kl (fst kl - 1, snd kl) _
+                                 L P l1 (a2 :: e1') t1' a3 /\
+                         a = a3
+                | _ => False
+              end)).
+  - assert (kl = (fst kl, snd kl)) by
+      (destruct kl; auto); rewrite H; simpl; clear H.
+    inversion _H; unfold pair_lt; auto.
+  - assert (kl = (fst kl, snd kl)) by
+      (destruct kl; auto); rewrite H; simpl; clear H.
+    inversion _H; unfold pair_lt; auto.
+  - assert (kl = (fst kl, snd kl)) by
+      (destruct kl; auto); rewrite H; simpl; clear H.
+    inversion _H; unfold pair_lt; auto.
+Defined.
+
+    (*| TDecl t1 t2 =>
+      match kl with
+        | (S k', l) =>
           exists e1' t1' l1 a2 v3 l3,
-            eval_k k' L P pc e t1 (Atom (VClos e1' t1') l1) /\
-            eval_k k' L P pc e t2 a2 /\
-            eval_k k' L P l1 (a2 :: e1') t1' (Atom v3 l3) /\
+            eval_kl (k', l) L P pc e t1 (Atom (VClos e1' t1') l1) /\
+            eval_kl (k', l) L P pc e t2 a2 /\
+            eval_kl (k', l) L P l1 (a2 :: e1') t1' (Atom v3 l3) /\
             match l3 with
               | Bottom2 =>
                 a = Atom v3 Bottom2
               | Top2 =>
                 (forall a2' e2' v3',
                    env_LPequiv L P (a2 :: e1') (a2' :: e2') ->
-                   eval_k k' L P l1 (a2' :: e2') t1' (Atom v3' Top2) ->
+                   eval_kl (l, k') L P l1 (a2' :: e2') t1' (Atom v3' Top2) ->
                    value_LPequiv L P v3 v3') /\
                 a = Atom v3 Bottom2
             end
-        | 0 => False
-      end
-  end.
+        | (0, _) => False
+      end*)
 
 Definition eval (L : two) (P : value -> value -> Prop)
            (pc : two) (e : env) (t : term) (a : atom) : Prop :=
-  forall k, eval_k k L P pc e t a.
+  exists k, forall l, eval_kl (k, l) L P pc e t a.
